Fix analysis stuff: Partial order now works with less or equal.
Previously, it required a less-than relation (which is not what we
want).

Compiler.v
@@ -54,38 +54,48 @@ Instance ToString_list : ToString (list var) := toString_list.
 
 Notation "S '<<' x '<<' y ';' s" := (let S := print_string S (x ++ "\n" ++ toString y ++ "\n\n") in s) (at level 1, left associativity).
 
-Definition ensure P `{Computable P} (s: string) : status unit :=
-if [P] then Success tt else Error s.
+Definition ensure_f P `{Computable P} (s: string) {A} (cont:status A) : status A :=
+if [P] then cont else Error s.
 
-Arguments ensure P [H] s.
+Arguments ensure_f P [H] s {A} cont.
+
+Notation "'ensure' P s ; cont " := (ensure_f P s cont)
+                                    (at level 20, P at level 0, s at level 0, cont at level 200, left associativity).
+
+(* Print Grammar operconstr. *)
 
 Definition toILF (ilin:ILN.nstmt) : status IL.stmt :=
   sdo ili <- ILN.labIndices ilin nil;
   sdo lv <- livenessAnalysis ili;
-  sdo _ <- ensure (Liveness.true_live_sound nil ili lv) "Liveness unsound";
+  ensure (Liveness.true_live_sound nil ili lv /\ getAnn lv ⊆ freeVars ili) ("Liveness unsound (1)") ;
   let ilid := DVE.compile nil ili lv in
   let additional_params := additionalArguments ilid (DVE.compile_live ili lv) in
-  sdo _ <- ensure (Delocation.trs nil nil ilid (DVE.compile_live ili lv) additional_params) "Liveness unsound";
+  ensure (Delocation.trs nil nil ilid (DVE.compile_live ili lv) additional_params)
+         "Additional arguments insufficient";
     Success (Delocation.compile nil ilid additional_params).
 
 
-Definition optimize (s:stmt) : status stmt :=
-  let s := rename_apart s in
+
+Definition optimize (s':stmt) : status stmt :=
+  let s := rename_apart s' in
   sdo ALAE <- constantPropagationAnalysis s;
   match ALAE with
-    | (AL, Some AE) =>
-      let s := ValueOpts.compile s
-                                (ConstantPropagation.cp_choose
-                                   (fun x => MapInterface.find x AE) s)
-      in
+    | (AL, AEc) =>
+      let AE := (fun x => MapInterface.find x AEc) in
+      ensure (ConstantPropagation.cp_sound AE nil s)
+             "Constant propagation unsound";
+      ensure (forall x, x ∈ freeVars s' -> AE x = None)
+             "Constant propagation makes no assumptions on free vars";
+      let s := ValueOpts.compile s (ConstantPropagation.cp_choose AE s) in
       sdo lv <- livenessAnalysis s;
-        Success (DVE.compile nil s lv)
-    | _ => Error "Constant propagation returned bottom"
+      ensure (Liveness.true_live_sound nil s lv) "Liveness unsound (2)";
+      Success (DVE.compile nil s lv)
   end.
-(*
+
+
 Definition fromILF (s:stmt) : status stmt :=
-  let s_renamed_apart := rename_apart s
-  in let lv := livenessAnalysis s_renamed_apart in
+  let s_renamed_apart := rename_apart s in
+  sdo lv <- livenessAnalysis s_renamed_apart;
      if [Liveness.live_sound nil s_renamed_apart lv
          /\ getAnn lv ⊆ freeVars s] then
        sdo ϱ <- allocation_oracle s_renamed_apart lv id;
@@ -98,7 +108,7 @@ Definition fromILF (s:stmt) : status stmt :=
          Error "Register allocation not injective."
      else
        Error "Liveness unsound.".
-*)
+
 Opaque LivenessValidators.live_sound_dec.
 Opaque DelocationValidator.trs_dec.
 
@@ -126,102 +136,184 @@ Proof.
 Qed.
 
 
-Lemma toILF_correct ilin s (E:onv val)
+Lemma toILF_correct (ilin:ILN.nstmt) s (E:onv val)
   : toILF ilin = Success s
-   -> @sim _ ILN.statetype_I _ _ (ILN.I.labenv_empty, E, ilin)
+    -> Delocation.defined_on (ILN.freeVars ilin) E
+    -> @sim _ ILN.statetype_I _ _ (ILN.I.labenv_empty, E, ilin)
           (nil:list F.block, E, s).
 Proof.
-  intros. unfold toILF in H. simpl in *; unfold ensure, additionalArguments in *.
+  intros. unfold toILF in H. simpl in *; unfold ensure_f, additionalArguments in *.
   monadS_inv H.
-  destruct if in EQ2; isabsurd.
-  destruct if in EQ0; isabsurd. clear x1 EQ0 EQ2 x2.
+  repeat (destruct if in EQ2; [|isabsurd]).
+  invc EQ2. dcr.
   eapply sim_trans with (S2:=I.state).
   - eapply bisim_sim. eapply ILN.labIndicesSim_sim.
     econstructor; eauto; isabsurd. econstructor; isabsurd.
   - case_eq (DelocationAlgo.computeParameters nil nil nil
               (DVE.compile nil x x0) (DVE.compile_live x x0)); intros.
-    assert (l = nil). admit. subst. eauto.
+    assert (l = nil). {
+    exploit (DelocationAlgo.computeParameters_length nil nil); eauto.
+    eapply (@DVE.dve_live nil); eauto. destruct l; simpl in *; congruence.
+    }
+    subst.
     exploit (@DVE.dve_live nil); eauto.
     exploit Delocation.trs_srd; eauto using PIR2.
     exploit (@DelocationAlgo.computeParameters_live nil nil nil); eauto using PIR2.
     eapply sim_trans with (S2:=I.state). Focus 2.
     eapply bisim_sim. eapply Bisim.bisim_sym.
-    rewrite H in X0.
+    rewrite H2 in X0.
     eapply Coherence.srdSim_sim; eauto.
     econstructor; eauto using AIR2. isabsurd. reflexivity.
-    simpl. rewrite H in t.
+    simpl. rewrite H2 in t.
     eapply (@Delocation.live_sound_compile nil nil nil); eauto.
 
     eapply sim_trans with (S2:=I.state).
     Focus 2.
     eapply bisim_sim. eapply Delocation.trsR_sim.
-    rewrite H in t.
+    rewrite H2 in t.
     econstructor; eauto using AIR53. reflexivity.
-    eapply (@Delocation.live_sound_compile nil); eauto. admit.
-    exfalso; admit.
-Admitted.
+    eapply (@Delocation.live_sound_compile nil); eauto.
+    hnf; intros. rewrite DVE.compile_live_incl in H3. eapply H0; eauto.
+    Lemma labIndices_freeVars ilin s L
+    : ILN.labIndices ilin L = Success s
+      -> ILN.freeVars ilin = freeVars s.
+    Proof.
+      intros. general induction ilin; simpl in *; monadS_inv H; simpl.
+      - erewrite IHilin; eauto.
+      - erewrite IHilin1, IHilin2; eauto.
+      - reflexivity.
+      - reflexivity.
+      - erewrite IHilin; eauto.
+      - erewrite IHilin1, IHilin2; try eapply EQ, EQ1; eauto.
+    Qed.
+    intros. erewrite labIndices_freeVars; eauto.
+    eauto.
+    eapply DVE.I.sim_DVE. reflexivity. eauto.
+Qed.
 
-(*
+
+Lemma fst_ssa_ann s G
+ : fst (getAnn (ssa_ann s G)) = G.
+Proof.
+  general induction s; eauto.
+Qed.
+
 Lemma fromILF_correct (s s':stmt) E
   : fromILF s = Success s'
   -> sim (nil:list F.block, E, s) (nil:list I.block, E, s').
 Proof.
   unfold fromILF; intros.
-  destruct if in H; dcr; isabsurd.
-  monadS_inv H; dcr. destruct if in EQ0.
+  monadS_inv H.
+  destruct if in EQ0; dcr; isabsurd.
+  monadS_inv EQ0; dcr. destruct if in EQ2; dcr.
   eapply sim_trans with (σ2:=(nil:list F.block, E, rename_apart s)).
+  eapply bisim_sim.
   eapply (@Alpha.alphaSim_sim (nil, E, s) (nil, E, rename_apart s)).
   econstructor; eauto using AIR3, Alpha.envCorr_idOn_refl.
   eapply Alpha.alpha_sym. eapply rename_apart_alpha.
   eapply sim_trans with (σ2:=(nil:list F.block, E,
-    rename x (rename_apart s))).
+    rename x0 (rename_apart s))).
+  eapply bisim_sim.
   eapply Alpha.alphaSim_sim. econstructor; eauto using AIR3.
-  eapply ssa_locally_inj_alpha; eauto.
+  eapply Allocation.ssa_locally_inj_alpha; eauto.
   eapply rename_apart_ssa; eauto; eapply lookup_set_on_id; try reflexivity.
-  eapply a.
-  instantiate (1:=id). destruct a.
-  eapply (@inverse_on_agree_on _ _ _ _ id x id id); try intuition.
-  eapply inverse_on_id.
-  hnf; intros. cbv in H2; subst. rewrite H2; eauto.
-  refine (sim_trans (Coherence.srdSim_sim _) (ParallelMove.pmSim_sim _)).
-  econstructor; isabsurd. eapply rename_ssa_srd; eauto.
-  eapply rename_apart_ssa; eauto. eapply a.
-  eapply I. econstructor.
-  eapply agree_on_refl.
+  instantiate (1:=id).
+  eapply (inverse_on_agree_on (inverse_on_id (G:=getAnn x))).
+  symmetry; eauto. reflexivity.
+  hnf; intros. cbv in H4; subst. rewrite H4; eauto.
+  eapply sim_trans with (S2:=I.state).
+  eapply bisim_sim.
+  eapply Coherence.srdSim_sim.
+  econstructor; isabsurd. eapply Allocation.rename_ssa_srd; eauto.
+  eapply rename_apart_ssa; eauto. rewrite fst_ssa_ann; eauto.
+  rewrite fst_ssa_ann; eauto.
+  eapply I. econstructor. reflexivity.
   eapply (@Liveness.live_rename_sound nil); eauto.
-  instantiate (1:=parallel_move).
-  econstructor; try eapply EQ0.
-  eapply (@Liveness.live_rename_sound nil); eauto.
-  constructor.
-  reflexivity.
+  eapply (ParallelMove.pmSim_sim).
+  econstructor; try now econstructor; eauto.
+  eapply (@Liveness.live_rename_sound nil); eauto. eauto.
   congruence.
 Qed.
-*)
+
+Lemma labelsDefined_rename_apart L s ϱ G
+: LabelsDefined.labelsDefined s L
+  -> LabelsDefined.labelsDefined (snd (rename_apart' ϱ G s)) L.
+Proof.
+  intros.
+  general induction H; simpl; repeat (let_pair_case_eq; simpl); try now econstructor; eauto; simpl_pair_eqs; instantiate; subst; eauto; subst.
+  - subst. exploit IHlabelsDefined; eauto. econstructor. eapply X.
+  - subst. econstructor.
+    + eapply IHlabelsDefined1; eauto.
+    + eapply IHlabelsDefined2; eauto.
+  - subst. econstructor. eapply IHlabelsDefined; eauto.
+  - subst. econstructor.
+    + eapply IHlabelsDefined1; eauto.
+    + eapply IHlabelsDefined2; eauto.
+Qed.
 
 Lemma optimize_correct (E:onv val) s s'
 : optimize s = Success s'
+  -> LabelsDefined.labelsDefined s 0
   -> sim (nil:list F.block, E, s) (nil:list F.block, E, s').
 Proof.
   intros.
-  unfold optimize in H.
-  (*
-  eapply (@sim_trans F.state _ F.state _).
-  instantiate (1:= (nil, E, DVE.compile s lv)).
-  admit.
-  eapply (@sim_trans F.state _ F.state _).
-  eapply CopyPropagation.subst_id.
-  eapply sim_sym.
-  eapply CopyPropagation.sim_CP.
+  unfold optimize, ensure_f in *.
+  monadS_inv H. destruct x.
+  repeat (destruct if in EQ0; [| isabsurd]).
+  monadS_inv EQ0.
+  repeat (destruct if in EQ2; [| isabsurd]).
+  invc EQ2.
+
+  eapply sim_trans with (S2:=F.state).
+  eapply bisim_sim.
+  eapply Alpha.alphaSim_sim. econstructor; eauto using rename_apart_alpha, AIR3.
+  eapply Alpha.alpha_sym. eapply rename_apart_alpha. hnf; intros.
+  cbv in H, H1. instantiate (1:=E). congruence.
+  eapply sim_trans with (S2:=F.state).
+  Focus 2.
+  eapply DVE.sim_DVE; eauto. reflexivity.
+  eapply sim'_sim.
+  eapply ValueOpts.sim_vopt; eauto.
+  Focus 2.
+  eapply ConstantPropagation.cp_sound_eqn; eauto.
+  eapply rename_apart_ssa. instantiate (1:=nil). simpl.
+  eapply labelsDefined_rename_apart; eauto.
+  intros; isabsurd.
+  rewrite fst_ssa_ann.
+  Lemma cp_eqns_no_assumption d G
+  : (forall x : var,
+      x \In G -> MapInterface.find x d = ⎣⎦)
+     -> ConstantPropagation.cp_eqns (fun x0 : var => MapInterface.find x0 d)
+        G [=] ∅.
+  Proof.
+    intros. revert H. pattern G. eapply set_induction.
+    intros. eapply empty_is_empty_1 in H. rewrite H.
+    reflexivity.
+    intros. eapply Add_Equal in H1. rewrite H1.
+    assert ({x; s} [=] {{x}} ∪ s) by (cset_tac; intuition).
+    rewrite H3. rewrite ConstantPropagation.cp_eqns_union.
+    rewrite ConstantPropagation.cp_eqns_single. unfold ConstantPropagation.cp_eqn.
+    rewrite H2. rewrite H. cset_tac; intuition. intros; eapply H2.
+    rewrite H1. cset_tac; intuition. rewrite H1. cset_tac; intuition.
+  Qed.
+  intros. hnf; intros.
+  rewrite cp_eqns_no_assumption in H. cset_tac; intuition. eassumption.
+  constructor.
+  eapply rename_apart_ssa.
+  rewrite fst_ssa_ann.
+  rewrite cp_eqns_no_assumption. eapply incl_empty. eauto.
+  hnf; intuition.
 Qed.
-*)
-Admitted.
 
 End Compiler.
 
-(*Print Assumptions toILF_correct.
-Print Assumptions fromILF_correct.*)
+Print Assumptions toILF_correct.
+Print Assumptions fromILF_correct.
+Print Assumptions optimize_correct.
+
 
 (* Unset Extraction AccessOpaque. *)
+
 
 Extraction Inline bind Option.bind toString.
 
