Libs/PartialOrder.v
@@ -2,8 +2,8 @@ Require Export Containers.OrderedType Setoid Coq.Classes.Morphisms Computable.
 Require Import Containers.OrderedTypeEx DecSolve MoreList.
 
 Class PartialOrder (Dom:Type) := {
-  poLt : Dom -> Dom -> Prop;
-  poLt_dec :> forall d d', Computable (poLt d d');
+  poLe : Dom -> Dom -> Prop;
+  poLe_dec :> forall d d', Computable (poLe d d');
   poEq : Dom -> Dom -> Prop;
   poEq_dec :> forall d d', Computable (poEq d d')
 }.
@@ -11,21 +11,21 @@ Class PartialOrder (Dom:Type) := {
 
 Instance PartialOrder_pair_instance X `{PartialOrder X} Y `{PartialOrder Y}
 : PartialOrder (X * Y) := {
-  poLt x y := poLt (fst x) (fst y) /\ poLt (snd x) (snd y);
-  poLt_dec := _;
+  poLe x y := poLe (fst x) (fst y) /\ poLe (snd x) (snd y);
+  poLe_dec := _;
   poEq x y := poEq (fst x) (fst y) /\ poEq (snd x) (snd y);
   poEq_dec := _
 }.
 - intros.
-  decide (poLt (fst d) (fst d')); decide (poLt (snd d) (snd d')); try dec_solve.
+  decide (poLe (fst d) (fst d')); decide (poLe (snd d) (snd d')); try dec_solve.
 - intros.
   decide (poEq (fst d) (fst d')); decide (poEq (snd d) (snd d')); try dec_solve.
 Defined.
 
 Instance PartialOrder_list_instance X `{PartialOrder X}
 : PartialOrder (list X) := {
-  poLt := list_eq poLt;
-  poLt_dec := _;
+  poLe := list_eq poLe;
+  poLe_dec := _;
   poEq := list_eq poEq;
   poEq_dec := _
 }.
